

1. (a) $a = b_i c_{ij} d_j \Rightarrow$ valid

(b) $a = b_i c_i + d_j \Rightarrow$ Invalid, free index "j" in only one term

(c) $a_i = \delta_{ij} b_i + c_i \Rightarrow$ Invalid as written since free index "j" only appears in one term

(d) $a_k = b_i c_{ki} \Rightarrow$ valid

(e) $a_k = b_k c + d_i e_{ik} \Rightarrow$ valid

(f) $a_i = b_i + c_{ij} d_{ji} e_i \Rightarrow$ Invalid, "i" is repeated three times in last term

(g) $a_l = \epsilon_{ijk} b_j c_k \Rightarrow$ Invalid, free index "l" does not match free index "i" on RHS

(h) $a_{ij} = b_{ji} \Rightarrow$ valid

(i) $a_{ij} = b_i c_j + e_{jk} \Rightarrow$ Invalid, free index "k" appears in only one term

(j) $a_{k\ell} = b_i c_{ki} d_\ell + e_{ki} \Rightarrow$ Invalid, free index "l" in first two terms does not appear in last term

2. (a) Prove $\delta_{ij} \delta_{ij} = 3$

ANSWER

$$\delta_{ij} \delta_{ij} = \sum_{i=1}^3 \sum_{j=1}^3 \delta_{ij} \delta_{ij} = \sum_{i=1}^3 [\delta_{i1}^2 + \delta_{i2}^2 + \delta_{i3}^2] = \begin{matrix} \delta_{11}^2 & \delta_{12}^2 & \delta_{13}^2 \\ \delta_{21}^2 & \delta_{22}^2 & \delta_{23}^2 \\ \delta_{31}^2 & \delta_{32}^2 & \delta_{33}^2 \end{matrix} = 1$$

Since $\delta_{ij} = 0$ for $i \neq j$ and $\delta_{ij} = 1$ for $i = j$,

$$\rightarrow \delta_{ij} \delta_{ij} = 3$$

2. (b) Prove $\epsilon_{pqr} \epsilon_{pqr} = 6$

ANSWER

$$\begin{aligned} \epsilon_{pqr} \epsilon_{pqr} &= \sum_{p=1}^3 \sum_{q=1}^3 \sum_{r=1}^3 \epsilon_{pqr} \epsilon_{pqr} = \sum_{p=1}^3 \left[\epsilon_{p1}^2 + \epsilon_{p2}^2 + \epsilon_{p3}^2 \right] \\ &= \sum_{p=1}^3 \left[\epsilon_{p11}^2 + \epsilon_{p12}^2 + \epsilon_{p13}^2 + \epsilon_{p21}^2 + \epsilon_{p22}^2 + \epsilon_{p23}^2 + \epsilon_{p31}^2 + \epsilon_{p32}^2 + \epsilon_{p33}^2 \right] \\ &= \epsilon_{112}^2 + \epsilon_{113}^2 + \epsilon_{121}^2 + \epsilon_{123}^2 + \epsilon_{131}^2 + \epsilon_{132}^2 \\ &\quad + \epsilon_{212}^2 + \epsilon_{213}^2 + \epsilon_{221}^2 + \epsilon_{223}^2 + \epsilon_{231}^2 + \epsilon_{232}^2 \\ &\quad + \epsilon_{312}^2 + \epsilon_{313}^2 + \epsilon_{321}^2 + \epsilon_{323}^2 + \epsilon_{331}^2 + \epsilon_{332}^2 \end{aligned}$$

$$\rightarrow \epsilon_{pqr} \epsilon_{pqr} = 6$$

3. Prove $\epsilon_{pqi} \epsilon_{paj} = 2 \delta_{ij}$

ANSWER

use epsilon-delta relation: $\epsilon_{ijk} \epsilon_{klm} = \delta_{il} \delta_{jm} - \delta_{im} \delta_{jl}$ (as given in textbook)

or, using the same indices as in the problem and realizing

that $\epsilon_{pqi} = \epsilon_{qip}$,

$$\epsilon_{pqi} \epsilon_{paj} = \epsilon_{qip} \epsilon_{paj} = \epsilon_{qjp} \epsilon_{paj} = \delta_{jq} \delta_{ip} - \delta_{jp} \delta_{iq} = 3 \delta_{ij} - \delta_{ij}$$

$$\rightarrow \epsilon_{pqi} \epsilon_{paj} = 2 \delta_{ij}$$

$$\begin{matrix} \epsilon_{pqi} \rightarrow \epsilon_{qip} \\ \downarrow \\ \epsilon_{qip} \end{matrix}$$

4. (a) Prove $\vec{u} \times \vec{v} = -\vec{v} \times \vec{u}$

ANSWER

LHS: $\vec{u} \times \vec{v} \Rightarrow \epsilon_{ijk} u_i v_j$

RHS: $-\vec{v} \times \vec{u} \Rightarrow -\epsilon_{ijk} v_i u_j = -\epsilon_{ijk} u_j v_i$

change indices on v and u to match those used on LHS: $i \rightarrow j, j \rightarrow i$

$$\Rightarrow -\epsilon_{jik} u_i v_j$$

now use identity, $-\epsilon_{jik} = \epsilon_{ijk}$

$$\Rightarrow \epsilon_{ijk} u_i v_j \quad \checkmark$$

4.(b) Show using index notation that

$$\vec{a} \times (\vec{b} \times \vec{c}) = (\vec{a} \cdot \vec{c}) \vec{b} - (\vec{a} \cdot \vec{b}) \vec{c}$$

ANSWER

let $\vec{d} = \vec{b} \times \vec{c}$. Then the left hand side is

Left-hand side: $LHS = \epsilon_{ijk} a_i d_j$ but $d_j = \epsilon_{lmj} b_l c_m$

$$= \epsilon_{ijk} \epsilon_{lmj} a_i b_l c_m$$

use epsilon-delta relation: $\epsilon_{ijk} \epsilon_{klm} = \delta_{il} \delta_{jm} - \delta_{im} \delta_{jl}$ (as given in book)

However, the repeating index is "k"; whereas in our problem, the repeating index is "j". Therefore, we switch "k" and "j" above:

$$\epsilon_{ikj} \epsilon_{jlm} = \delta_{il} \delta_{jm} - \delta_{im} \delta_{jl}$$

Now, we have to get the order of the indices to match that in our problem. we realize that

$$\epsilon_{ikj} = -\epsilon_{ijk} \quad \text{and} \quad \epsilon_{jlm} = \epsilon_{lmj}$$

Now, we go back to our problem ...

$$= -\epsilon_{ikj} \epsilon_{jlm} a_i b_l c_m = -(\underbrace{\delta_{il} \delta_{jm} - \delta_{im} \delta_{jl}}_{\text{two terms}}) a_i b_l c_m$$

$$= \delta_{im} \delta_{jl} a_i b_l c_m - \delta_{il} \delta_{jm} a_i b_l c_m$$

$$= b_j \underbrace{a_i c_i}_{\vec{a} \cdot \vec{c}} - c_j \underbrace{a_l b_l}_{\vec{a} \cdot \vec{b}}$$

$$= (\vec{a} \cdot \vec{c}) \vec{b} - (\vec{a} \cdot \vec{b}) \vec{c} \quad \checkmark$$

4.(c) Prove $\underbrace{(\vec{a} \times \vec{b}) \cdot \vec{c}}_{\text{I}} = \underbrace{\vec{a} \cdot (\vec{b} \times \vec{c})}_{\text{II}} = \underbrace{(\vec{c} \times \vec{a}) \cdot \vec{b}}_{\text{III}}$

ANSWER

Term I: $(\vec{a} \times \vec{b}) \cdot \vec{c} \Rightarrow (\epsilon_{ijk} a_i b_j) c_k = \epsilon_{ijk} a_i b_j c_k$

Term II: $\vec{a} \cdot (\vec{b} \times \vec{c}) \Rightarrow \epsilon_{ijk} b_i c_j a_k$

now rewrite indices on b, c, a to match that of Term I, i.e., change $k \rightarrow i, j \rightarrow k, i \rightarrow j$

$$\Rightarrow \epsilon_{jki} a_i b_j c_k = \epsilon_{ijk} a_i b_j c_k \quad \checkmark$$

use $\epsilon_{jki} = \epsilon_{ijk}$

Term III: $(\vec{c} \times \vec{a}) \cdot \vec{b} \Rightarrow (\epsilon_{ijk} c_i a_j) b_k$

change indices to match those above: $i \rightarrow k, j \rightarrow i, k \rightarrow j$

$$\Rightarrow \epsilon_{kij} a_i b_j c_k = \epsilon_{ijk} a_i b_j c_k \quad \checkmark$$

$\epsilon_{kij} = \epsilon_{ijk}$

5. Prove $\vec{\nabla} \cdot (\vec{\nabla} \times \vec{u}) = 0$ for any arbitrary vector \vec{u} .

ANSWER

First we write the term in parenthesis using index notation

$$\vec{\nabla} \times \vec{u} \Rightarrow \epsilon_{ijk} \frac{\partial u_k}{\partial x_j}$$

Now take divergence recognizing that $\vec{\nabla} \cdot \vec{a} = \frac{\partial a_i}{\partial x_i}$

$$\vec{\nabla} \cdot (\vec{\nabla} \times \vec{u}) \Rightarrow \frac{\partial}{\partial x_i} \left(\epsilon_{ijk} \frac{\partial u_k}{\partial x_j} \right) = \epsilon_{ijk} \frac{\partial^2 u_k}{\partial x_i \partial x_j}$$

However, since "i" and "j" are just dummy (repeated) indices, we can swap them without changing the result. Therefore,

$$\epsilon_{ijk} \frac{\partial^2 u_k}{\partial x_i \partial x_j} = \epsilon_{jik} \frac{\partial^2 u_k}{\partial x_j \partial x_i} = \epsilon_{jik} \frac{\partial^2 u_k}{\partial x_i \partial x_j}$$

swap "i" & "j" order of differentiation does not matter

Now recall that $\epsilon_{jik} = -\epsilon_{ijk}$, so

$$\epsilon_{ijk} \frac{\partial^2 u_k}{\partial x_i \partial x_j} = -\epsilon_{ijk} \frac{\partial^2 u_k}{\partial x_i \partial x_j}$$

→ The only way that a quantity can equal the negative value of itself is if that quantity is zero.